Quotation up through Kernames

theories/Template/QuoteGround/Init.v
@@ -9,9 +9,24 @@ Class quotation_of {T} (t : T) := quoted_term_of : Ast.term.
 Class ground_quotable T := quote_ground : forall t : T, quotation_of t.
 Class debug_opt := debug : bool.
 
-Fixpoint replace_quotation_of {debug : debug_opt} (qt : term) : TemplateMonad term.
+(* returns true if a modpath is suitable for quotation, i.e., does not mention functor-bound arguments *)
+Fixpoint modpath_is_absolute (mp : modpath) : bool
+  := match mp with
+     | MPfile _ => true
+     | MPbound _ _ _ => false
+     | MPdot mp _ => modpath_is_absolute mp
+     end.
+(* returns false iff a term is suitable for quotation at the top-level, i.e., returns true iff it mentions functor-bound arguments or is a local variable *)
+Definition head_term_is_bound (t : term) : bool
+  := match t with
+     | tConst (kn, _) _ => negb (modpath_is_absolute kn)
+     | tVar _ => true
+     | _ => false
+     end.
+
+Fixpoint replace_quotation_of' {debug : debug_opt} (qt : term) : TemplateMonad term.
 Proof.
-  specialize (replace_quotation_of debug).
+  specialize (replace_quotation_of' debug).
   simple
     refine
     (let tmInferQuotation t
@@ -22,37 +37,46 @@ Proof.
            | my_Some v => tmReturn v
            | my_None => (if debug then tmPrint (quotation_of t) else tmReturn tt);; tmFail "No typeclass instance"
            end) in
-     match qt return TemplateMonad Ast.term with
-     | tRel _
-     | tSort _
-     | tConstruct _ _ _
-     | tInt _
-     | tFloat _
-     | tConst _ _
-     | tInd _ _
-       => ret qt
-     | tVar id
-       => tmInferQuotation qt
-     | tEvar ev args => args <- monad_map replace_quotation_of args;; ret (tEvar ev args)
-     | tLambda na T M => T <- replace_quotation_of T;; M <- replace_quotation_of M;; ret (tLambda na T M)
-     | tApp u v => u <- replace_quotation_of u;; v <- monad_map replace_quotation_of v;; ret (mkApps u v)
-     | tProd na A B => A <- replace_quotation_of A;; B <- replace_quotation_of B;; ret (tProd na A B)
-     | tCast c kind ty => c <- replace_quotation_of c;; ty <- replace_quotation_of ty;; ret (tCast c kind ty)
-     | tLetIn na b ty b' => b <- replace_quotation_of b;; ty <- replace_quotation_of ty;; b' <- replace_quotation_of b';; ret (tLetIn na b ty b')
-     | tProj p c => replace_quotation_of c;; ret (tProj p c)
-     | tFix mfix idx =>
-         mfix' <- monad_map (monad_map_def (TM:=TypeInstance) replace_quotation_of replace_quotation_of) mfix;;
-         ret (tFix mfix' idx)
-     | tCoFix mfix idx =>
-         mfix' <- monad_map (monad_map_def (TM:=TypeInstance) replace_quotation_of replace_quotation_of) mfix;;
-         ret (tCoFix mfix' idx)
-     | tCase ind p c brs =>
-         p' <- monad_map_predicate (TM:=TypeInstance) ret replace_quotation_of replace_quotation_of p;;
-         brs' <- monad_map_branches (TM:=TypeInstance) replace_quotation_of brs;;
-         c <- replace_quotation_of c;;
-         ret (tCase ind p' c brs')
-     end); exact _.
+     if head_term_is_bound qt
+     then tmInferQuotation qt
+     else
+       match qt return TemplateMonad Ast.term with
+       | tRel _
+       | tSort _
+       | tConstruct _ _ _
+       | tInt _
+       | tFloat _
+       | tConst _ _
+       | tInd _ _
+         => ret qt
+       | tVar _
+         => tmInferQuotation qt
+       | tEvar ev args => args <- monad_map replace_quotation_of' args;; ret (tEvar ev args)
+       | tLambda na T M => T <- replace_quotation_of' T;; M <- replace_quotation_of' M;; ret (tLambda na T M)
+       | tApp u v => u <- replace_quotation_of' u;; v <- monad_map replace_quotation_of' v;; ret (mkApps u v)
+       | tProd na A B => A <- replace_quotation_of' A;; B <- replace_quotation_of' B;; ret (tProd na A B)
+       | tCast c kind ty => c <- replace_quotation_of' c;; ty <- replace_quotation_of' ty;; ret (tCast c kind ty)
+       | tLetIn na b ty b' => b <- replace_quotation_of' b;; ty <- replace_quotation_of' ty;; b' <- replace_quotation_of' b';; ret (tLetIn na b ty b')
+       | tProj p c => replace_quotation_of' c;; ret (tProj p c)
+       | tFix mfix idx =>
+           mfix' <- monad_map (monad_map_def (TM:=TypeInstance) replace_quotation_of' replace_quotation_of') mfix;;
+           ret (tFix mfix' idx)
+       | tCoFix mfix idx =>
+           mfix' <- monad_map (monad_map_def (TM:=TypeInstance) replace_quotation_of' replace_quotation_of') mfix;;
+           ret (tCoFix mfix' idx)
+       | tCase ind p c brs =>
+           p' <- monad_map_predicate (TM:=TypeInstance) ret replace_quotation_of' replace_quotation_of' p;;
+           brs' <- monad_map_branches (TM:=TypeInstance) replace_quotation_of' brs;;
+           c <- replace_quotation_of' c;;
+           ret (tCase ind p' c brs')
+       end); exact _.
 Defined.
+
+Definition replace_quotation_of {debug : debug_opt} {T} (t : T) : TemplateMonad term
+  := qt <- tmQuote t;;
+     if head_term_is_bound qt
+     then tmFail "Avoiding loops"
+     else replace_quotation_of' qt.
 
 (** for fancier goals when we have [ground_quotable] for some subterms but not for subterms of those subterms *)
 Definition make_quotation_of {debug : debug_opt} {T} (t : T) : TemplateMonad (quotation_of t).
@@ -62,51 +86,53 @@ Proof.
     (qt <- tmQuote t;;
      let tmInferQuotation t
        := (t <- tmUnquote t;;
-           v <- (let '(existT_typed_term _ t) := t in tmInferInstance None (quotation_of t));;
+           let '(existT_typed_term _ t) := t in
+           v <- tmInferInstance None (quotation_of t);;
            match v with
            | my_Some v => tmReturn v
            | my_None => (if debug then tmPrint (quotation_of t) else tmReturn tt);; tmFail "No typeclass instance"
            end) in
-     match qt return TemplateMonad Ast.term with
-     | tSort _
-     | tConst _ _
-     | tConstruct _ _ _
-     | tInt _
-     | tFloat _
-     | tInd _ _
-       => tmReturn qt
-     | tCast t kind v
-       => tmInferQuotation t
-     | tApp f args
-       => qf <- tmInferQuotation f;;
-          qargs <- list_rect
-                     (fun _ => _)
-                     (tmReturn [])
-                     (fun arg args qargs
-                      => qarg <- tmInferQuotation arg;;
-                         qargs <- qargs;;
-                         tmReturn (qarg :: qargs))
-                     args;;
-          tmReturn (tApp qf qargs)
-     | tProj proj t => tmFail "Proj is not reduced"
-     | tRel n => tmFail "Rel is not ground"
-     | tVar id => tmFail "Var is not ground"
-     | tEvar ev args => tmFail "Evar is not ground"
-     | tProd na ty body => tmFail "Prod not yet handled"
-     | tLambda na ty body => tmFail "Lambda not yet handled"
-     | tLetIn na def def_ty body => tmFail "LetIn not yet handled"
-     | tCase ci type_info discr branches => tmFail "Case not yet handled"
-     | tFix mfix idx => tmFail "Fix not yet handled"
-     | tCoFix mfix idx => tmFail "CoFix not yet handled"
-     end);
+     if head_term_is_bound qt
+     then tmFail "bound argument is not ground"
+     else
+       match qt return TemplateMonad Ast.term with
+       | tSort _
+       | tConst _ _
+       | tConstruct _ _ _
+       | tInt _
+       | tFloat _
+       | tInd _ _
+         => tmReturn qt
+       | tCast t kind v
+         => tmInferQuotation t
+       | tApp f args
+         => qf <- tmInferQuotation f;;
+            qargs <- list_rect
+                       (fun _ => _)
+                       (tmReturn [])
+                       (fun arg args qargs
+                        => qarg <- tmInferQuotation arg;;
+                           qargs <- qargs;;
+                           tmReturn (qarg :: qargs))
+                       args;;
+            tmReturn (tApp qf qargs)
+       | tProj proj t => tmFail "Proj is not reduced"
+       | tRel n => tmFail "Rel is not ground"
+       | tVar id => tmFail "Var is not ground"
+       | tEvar ev args => tmFail "Evar is not ground"
+       | tProd na ty body => tmFail "Prod not yet handled"
+       | tLambda na ty body => tmFail "Lambda not yet handled"
+       | tLetIn na def def_ty body => tmFail "LetIn not yet handled"
+       | tCase ci type_info discr branches => tmFail "Case not yet handled"
+       | tFix mfix idx => tmFail "Fix not yet handled"
+       | tCoFix mfix idx => tmFail "CoFix not yet handled"
+       end);
     exact _.
 Defined.
 
 Ltac replace_quotation_of_goal _ :=
-  let G := match goal with |- quotation_of ?G => G end in
-  tryif is_var G
-  then fail "Avoiding loops"
-  else run_template_program (replace_quotation_of <% G %>) (fun v => exact v).
+  let t := match goal with |- quotation_of ?t => t end in
+  run_template_program (replace_quotation_of t) (fun v => exact v).
 
 Ltac make_quotation_of_goal _ :=
   let t := match goal with |- quotation_of ?t => t end in
