theories/Template/QuoteGround/Coq/FSets.v
@@ -1,0 +1,206 @@
+From Coq Require Import FMapInterface FMapList FMapAVL FMapFullAVL FMapFacts.
+From MetaCoq.Lob.Template.QuoteGround Require Export Coq.Numbers Coq.Init Coq.Lists.
+From MetaCoq.Lob.Util.Tactics Require Import
+     SplitInContext
+     SpecializeBy
+     SpecializeAllWays
+     DestructHead
+     SpecializeUnderBindersBy
+     InHypUnderBindersDo
+     BreakMatch
+.
+
+Module QuoteWSfun (E : DecidableType) (Import W : WSfun E).
+  Module Import WFacts := WFacts_fun E W.
+
+  Section with_quote.
+    Context {elt : Type}
+            {qE_t : quotation_of E.t} {qelt : quotation_of elt} {qt : quotation_of t}
+            {qMapsTo : quotation_of MapsTo}
+            {qfind : quotation_of find} {qmem : quotation_of mem} {qelements : quotation_of elements}
+            {qfind_mapsto_iff : quotation_of find_mapsto_iff}.
+
+    #[export] Instance qIn : quotation_of In := ltac:(cbv [In]; exact _).
+    #[export] Instance qEmpty : quotation_of Empty := ltac:(cbv [Empty]; exact _).
+    #[export] Instance qEqual : quotation_of (@Equal) := ltac:(cbv -[quotation_of]; exact _).
+    #[export] Instance qEquiv : quotation_of (@Equiv) := ltac:(cbv -[quotation_of]; exact _).
+
+    #[export] Instance quote_MapsTo {x y z} {qx : quotation_of x} {qy : quotation_of y} {qz : quotation_of z} : ground_quotable (@MapsTo elt x y z)
+        := quote_of_iff (iff_sym (@find_mapsto_iff _ _ _ _)).
+
+    #[export] Instance quote_In {k m} {qk : quotation_of k} {qm : quotation_of m} : ground_quotable (@In elt k m)
+      := quote_of_iff (iff_sym (@mem_in_iff _ _ _)).
+    #[export] Instance quote_neg_In {k m} {qk : quotation_of k} {qm : quotation_of m} : ground_quotable (~@In elt k m)
+      := quote_neg_of_iff (iff_sym (@mem_in_iff _ _ _)).
+
+    #[export] Instance quote_Empty {m} {qm : quotation_of m} : ground_quotable (@Empty elt m)
+      := quote_of_iff (iff_sym (@is_empty_iff _ _)).
+    #[export] Instance quote_neg_Empty {m} {qm : quotation_of m} : ground_quotable (~@Empty elt m)
+      := quote_neg_of_iff (iff_sym (@is_empty_iff _ _)).
+
+    Definition Equiv_alt (eq_elt : elt -> elt -> Prop) m m' :=
+      let eq_opt_elt x y := match x, y with
+                            | Some x, Some y => eq_elt x y
+                            | None, None => True
+                            | Some _, None | None, Some _ => False
+                            end in
+      List.Forall (fun '(k, _) => eq_opt_elt (find k m) (find k m')) (@elements elt m)
+      /\ List.Forall (fun '(k, _) => eq_opt_elt (find k m) (find k m')) (@elements elt m').
+    #[local] Hint Extern 1 => break_innermost_match_step : typeclass_instances.
+    #[export] Instance quote_Equiv_alt {eq_elt} {m m'} {qeq_elt : quotation_of eq_elt} {quote_elt : ground_quotable elt} {quote_key : ground_quotable key} {quote_eq_elt : forall x y, ground_quotable (eq_elt x y:Prop)} {qm : quotation_of m} {qm' : quotation_of m'} : ground_quotable (@Equiv_alt eq_elt m m') := _.
+    Lemma Equiv_alt_iff {eq_elt m m'} : Equiv_alt eq_elt m m' <-> Equiv eq_elt m m'.
+    Proof using Type.
+      cbv [Equiv Equiv_alt].
+      cbv [In] in *.
+      setoid_rewrite find_mapsto_iff.
+      rewrite !Forall_forall.
+      pose proof (@find_o elt m).
+      pose proof (@find_o elt m').
+      transitivity
+        (let eq_opt_elt x y := match x, y with
+                               | Some x, Some y => eq_elt x y
+                               | None, None => True
+                               | Some _, None | None, Some _ => False
+                               end in
+         (forall k, In k m -> eq_opt_elt (find k m) (find k m'))
+         /\ (forall k, In k m' -> eq_opt_elt (find k m) (find k m'))).
+      1: cbv [In]; setoid_rewrite elements_mapsto_iff; setoid_rewrite InA_alt; cbv [eq_key_elt]; cbn [fst snd].
+      2: cbv [In]; setoid_rewrite find_mapsto_iff.
+      all: repeat (split || intros || destruct_head'_and || split_iff || destruct_head'_prod || destruct_head'_ex || subst).
+      all: specialize_dep_under_binders_by eapply ex_intro.
+      all: specialize_dep_under_binders_by eapply conj.
+      all: specialize_dep_under_binders_by eapply eq_refl.
+      all: specialize_dep_under_binders_by eapply pair.
+      all: cbn [fst snd] in *.
+      all: specialize_all_ways_under_binders_by apply E.eq_refl.
+      all: repeat first [ progress destruct_head'_ex
+                        | match goal with
+                          | [ H : List.In _ _ |- _ ]
+                            => progress specialize_under_binders_by exact H
+                          | [ H : E.eq _ _ |- _ ]
+                            => progress specialize_under_binders_by exact H
+                          | [ H : find _ _ = Some _ |- _ ]
+                            => progress specialize_under_binders_by exact H
+                          end ].
+      all: try solve [ break_innermost_match; break_innermost_match_hyps; try congruence; eauto ].
+    Qed.
+
+    #[export] Instance quote_Equiv {eq_elt m m'} {qm : quotation_of m} {qm' : quotation_of m'} {quote_elt : ground_quotable elt} {quote_key : ground_quotable key} {qeq_elt : quotation_of eq_elt} {quote_eq_elt : forall x y, ground_quotable (eq_elt x y:Prop)} : ground_quotable (@Equiv elt eq_elt m m') := quote_of_iff Equiv_alt_iff.
+
+    #[export] Instance quote_Equal {m m'} {qm : quotation_of m} {qm' : quotation_of m'} {quote_elt : ground_quotable elt} {quote_key : ground_quotable key} : ground_quotable (@Equal elt m m') := quote_of_iff (iff_sym (@Equal_Equiv elt m m')).
+
+    #[export] Instance quote_Equivb {cmp m m'} {qm : quotation_of m} {qm' : quotation_of m'} {quote_elt : ground_quotable elt} {quote_key : ground_quotable key} {qcmp : quotation_of cmp} : ground_quotable (@Equivb elt cmp m m') := _.
+  End with_quote.
+
+  Module Export Instances.
+    #[export] Existing Instances
+     qIn
+     qEmpty
+     qEqual
+     qEquiv
+     quote_MapsTo
+     quote_In
+     quote_neg_In
+     quote_Empty
+     quote_neg_Empty
+     quote_Equiv_alt
+     quote_Equiv
+     quote_Equal
+     quote_Equivb
+    .
+  End Instances.
+End QuoteWSfun.
+
+
+Module Type FMapAVL_MakeT (T : OrderedType). Include FMapAVL.Make T. End FMapAVL_MakeT.
+
+Module QuoteFMapAVL (T : OrderedType) (M : FMapAVL_MakeT T).
+  Module Import QM := QuoteWSfun T M.
+
+  Scheme Induction for M.Raw.tree Sort Type.
+  Scheme Induction for M.Raw.tree Sort Set.
+  Scheme Induction for M.Raw.tree Sort Prop.
+  Scheme Case for M.Raw.tree Sort Type.
+  Scheme Case for M.Raw.tree Sort Prop.
+  Scheme Minimality for M.Raw.tree Sort Type.
+  Scheme Minimality for M.Raw.tree Sort Set.
+  Scheme Minimality for M.Raw.tree Sort Prop.
+
+  Section with_t.
+    Context {elt : Type}
+            {qelt : quotation_of elt}
+            {quote_elt : ground_quotable elt} {quote_T_t : ground_quotable T.t}.
+
+    #[export] Instance quote_M_Raw_t : ground_quotable (M.Raw.t elt) := (ltac:(induction 1; exact _)).
+    Fixpoint M_Raw_lt_tree_dec x t : { @M.Raw.lt_tree elt x t } + {~ @M.Raw.lt_tree elt x t}.
+    Proof.
+      refine match t with
+             | M.Raw.Leaf => left _
+             | M.Raw.Node l k n r z
+               => match T.compare k x, M_Raw_lt_tree_dec x l, M_Raw_lt_tree_dec x r with
+                  | LT p1, left p2, left p3 => left _
+                  | _, right pf, _ => right _
+                  | _, _, right pf => right _
+                  | _, _, _ => right _
+                  end
+             end;
+        try solve [ inversion 1
+                  | inversion 1; subst; auto;
+                    match goal with
+                    | [ H : T.lt _ _, H' : T.eq _ _ |- _ ]
+                      => now first [ rewrite -> H' in H | rewrite <- H' in H ]
+                    end
+                  | intro f; apply pf; hnf in *; intros; apply f; constructor; (assumption + reflexivity)
+                  | intro f; eapply M.Raw.Proofs.MX.lt_antirefl; (idtac + etransitivity); (eassumption + (eapply f; constructor; (idtac + symmetry); (eassumption + reflexivity))) ].
+    Defined.
+    Fixpoint M_Raw_gt_tree_dec x t : { @M.Raw.gt_tree elt x t } + {~ @M.Raw.gt_tree elt x t}.
+    Proof.
+      refine match t with
+             | M.Raw.Leaf => left _
+             | M.Raw.Node l k n r z
+               => match T.compare k x, M_Raw_gt_tree_dec x l, M_Raw_gt_tree_dec x r with
+                  | GT p1, left p2, left p3 => left _
+                  | _, right pf, _ => right _
+                  | _, _, right pf => right _
+                  | _, _, _ => right _
+                  end
+             end;
+        try solve [ inversion 1
+                  | inversion 1; subst; auto;
+                    match goal with
+                    | [ H : T.lt _ _, H' : T.eq _ _ |- _ ]
+                      => now first [ rewrite -> H' in H | rewrite <- H' in H ]
+                    end
+                  | intro f; apply pf; hnf in *; intros; apply f; constructor; (assumption + reflexivity)
+                  | intro f; eapply M.Raw.Proofs.MX.lt_antirefl; (idtac + etransitivity); (eassumption + (eapply f; constructor; (idtac + symmetry); (eassumption + reflexivity))) ].
+    Defined.
+    Fixpoint M_Raw_bst_dec t : { @M.Raw.bst elt t } + {~ @M.Raw.bst elt t}.
+    Proof.
+      refine match t with
+             | M.Raw.Leaf => left _
+             | M.Raw.Node l k n r z
+               => match M_Raw_bst_dec l, M_Raw_bst_dec r, M_Raw_lt_tree_dec k l, M_Raw_gt_tree_dec k r with
+                  | right pf, _, _, _ => right _
+                  | _, right pf, _, _ => right _
+                  | _, _, right pf, _ => right _
+                  | _, _, _, right pf => right _
+                  | left p1, left p2, left p3, left p4 => left _
+                  end
+             end;
+        try solve [ constructor; assumption
+                  | inversion 1; subst; auto ].
+    Defined.
+    #[export] Instance quote_Raw_bst t : ground_quotable (M.Raw.bst t)
+      := ground_quotable_of_dec (@M_Raw_bst_dec t).
+    #[export] Instance quote_t : ground_quotable (M.t elt) := (ltac:(induction 1; exact _)).
+  End with_t.
+
+  Module Export Instances.
+    Export QM.Instances.
+    #[export] Existing Instances
+     quote_M_Raw_t
+     quote_Raw_bst
+     quote_t
+    .
+  End Instances.
+End QuoteFMapAVL.
