theories/Template/QuoteGround/Coq/Init.v
@@ -11,7 +11,9 @@ Export QuoteGround.Init.Instances.
 #[export] Instance quote_unit : ground_quotable unit := ltac:(destruct 1; exact _).
 #[export] Instance quote_bool : ground_quotable bool := ltac:(destruct 1; exact _).
 
-#[export] Instance quote_eq {A} {qA : quotation_of A} {qA : ground_quotable A} {x y : A} : ground_quotable (x = y :> A) := (ltac:(intros []; exact _)).
+#[export] Instance quote_eq {A} {qA : quotation_of A} {qA : ground_quotable A} {x y : A} : ground_quotable (x = y :> A) := ltac:(intros []; exact _).
+#[export] Instance quote_eq_refl_l {A} {qA : quotation_of A} {x y : A} {qx : quotation_of x} : ground_quotable (x = y :> A) := ltac:(intros []; exact _).
+#[export] Instance quote_eq_refl_r {A} {qA : quotation_of A} {x y : A} {qy : quotation_of y} : ground_quotable (x = y :> A) := ltac:(intro; subst; exact _).
 
 Definition ground_quotable_of_bp {b P} (H : b = true -> P) {qH : quotation_of H} (H_for_safety : P -> b = true) : ground_quotable P.
 Proof.
