theories/Template/QuoteGround/Kernames.v
@@ -1,0 +1,13 @@
+From MetaCoq.Lob.Template.QuoteGround Require Export Coq.Init Coq.MSets Coq.FSets bytestring.
+From MetaCoq.Template Require Import Kernames.
+
+#[export] Instance quote_modpath : ground_quotable modpath := ltac:(induction 1; exact _).
+
+Module QuoteKernameSet := QuoteMSetAVL Kername KernameSet.
+Export QuoteKernameSet.Instances.
+Module QuoteKernameMap := QuoteFMapAVL Kername.OT KernameMap.
+Export QuoteKernameMap.Instances.
+
+#[export] Instance quote_inductive : ground_quotable inductive := ltac:(destruct 1; exact _).
+#[export] Instance quote_projection : ground_quotable projection := ltac:(destruct 1; exact _).
+#[export] Instance quote_global_reference : ground_quotable global_reference := ltac:(destruct 1; exact _).
