theories/Template/QuoteGround/utils/wGraph.v
@@ -23,8 +23,17 @@ Module QuoteWeightedGraph (V : UsualOrderedType) (VSet : MSetInterface.S with Mo
   Module Import QuoteEdgeSet := QuoteMSetAVL Edge EdgeSet.
 
   Section with_quote.
-    Context {qV_t : quotation_of V.t} {qVSet_t : quotation_of VSet.t}
+    Context {qEdgeSet_t : quotation_of EdgeSet.t} {qV_t : quotation_of V.t} {qVSet_t : quotation_of VSet.t}
+            {qVSet_In : quotation_of VSet.In} {qEdgeSet_In : quotation_of EdgeSet.In}
+            {qVSet_eq_dec : quotation_of VSet.eq_dec} {qVSet_add : quotation_of VSet.add} {qEdgeSet_subset_spec : quotation_of EdgeSet.subset_spec} {qlsp : quotation_of lsp}
             {quote_V_t : ground_quotable V.t} {quote_VSet_t : ground_quotable VSet.t}.
+
+    #[export] Instance qEdgeSet_elt : quotation_of EdgeSet.elt := ltac:(cbv -[quotation_of]; exact _).
+    #[export] Instance qt : quotation_of t := ltac:(cbv [t]; exact _).
+    #[export] Instance qWE : quotation_of W.E := ltac:(cbv [W.E]; exact _).
+    #[export] Instance qWV : quotation_of W.V := ltac:(cbv [W.V]; exact _).
+    #[export] Instance qVSetProp_Add : quotation_of VSetProp.Add := ltac:(cbv [VSetProp.Add]; exact _).
+    #[export] Instance qVSet : quotation_of VSetProp.Add := ltac:(cbv [VSetProp.Add]; exact _).
 
     #[export] Instance quote_PathOf {G x y} : ground_quotable (@PathOf G x y) := ltac:(induction 1; exact _).
     #[export] Instance quote_SPath {G s x y} : ground_quotable (@SPath G s x y) := ltac:(induction 1; exact _).
@@ -42,7 +51,13 @@ Module QuoteWeightedGraph (V : UsualOrderedType) (VSet : MSetInterface.S with Mo
                 eapply Edge.lt_strorder; (idtac + etransitivity); eassumption ].
     Defined.
 
-    #[export] Instance quote_lt {x y} {qx : quotation_of x} {qy : quotation_of y} : ground_quotable (Edge.lt x y) := ground_quotable_of_dec (@lt_dec x y).
+    Section with_quote.
+      Context {qV_t : quotation_of V.t} {qV_lt : quotation_of V.lt}.
+
+      #[export] Instance qEdge_t : quotation_of Edge.t := ltac:(cbv -[quotation_of]; exact _).
+      #[export] Instance qlt : quotation_of Edge.lt := ltac:(cbv [Edge.lt V.eq]; try exact _).
+      #[export] Instance quote_lt {x y} {qx : quotation_of x} {qy : quotation_of y} : ground_quotable (Edge.lt x y) := ground_quotable_of_dec (@lt_dec x y).
+    End with_quote.
 
     Module Export Instances.
       #[export] Existing Instances
