theories/Util/Tactics/SpecializeAllWays.v
@@ -1,0 +1,7 @@
+Require Export MetaCoq.Lob.Util.Tactics.UniquePose.
+
+Ltac specialize_all_ways :=
+  repeat match goal with
+         | [ H : ?A, H' : forall a : ?A, _ |- _ ]
+           => unique pose proof (H' H)
+         end.
