theories/Util/Tactics/Zeta1.v
@@ -1,0 +1,6 @@
+Require Export MetaCoq.Lob.Util.Notations.
+
+Ltac zeta1 x :=
+  lazymatch x with
+  | let a := ?b in ?f => constr:(subst_let a := b in f)
+  end.
