theories/Util/Notations.v
@@ -1,0 +1,4 @@
+Reserved Notation "'subst_let' x := y 'in' z"
+         (at level 200, z at level 200, format "'subst_let'  x  :=  y  'in' '//' z").
+
+Notation "'subst_let' x := y 'in' z" := (match y return _ with x => z end) (only parsing).
